clean up

theories/EndpointTree.v
@@ -88,74 +88,6 @@ intros. rewrite /idemp. intros. rewrite {2}/full_eunf. rewrite full_eunf2. done.
 Qed.
 
 
-
-
-(*
-Fixpoint muv n g := 
-match g with 
-| ERec g0 => muv n.+1 g0
-| EVar n0 => n == n0
-| _ => false 
-end. 
-
-Lemma not_eguarded_muv : forall g n, ~~ eguarded n g -> muv n g. 
-Proof. 
-elim=>//=;intros; solve [ lia | auto].   
-Qed.
-
-
-Lemma not_eguarded_muv2 : forall g n,  muv n g -> ~~ eguarded n g.
-Proof. 
-elim=>//=;intros; solve [ lia | auto].   
-Qed.
-
-
-Lemma muv_uniq : forall g n0 n1, muv n0 g -> muv n1 g -> n0 = n1. 
-Proof. 
-elim=>//=. 
-intros. lia. 
-intros. suff : n0.+1 = n1.+1.  lia. apply/H=>//=. 
-Qed.
-
-Lemma muv_ren : forall g n sigma, muv n g -> muv (sigma n) g ⟨e sigma ⟩.
-Proof. simpl. 
-elim=>//=;intros. 
-move/eqP : H=>Heq. subst=>//=. 
-asimpl. apply (@H _  (0 .: sigma >> succn)) in H0. 
-move : H0. asimpl=>//=. 
-Qed.
-
-
-
-Lemma muv_subst : forall g n n0 sigma, muv n (sigma n0) -> muv n0 g -> muv n g[e sigma].
-Proof. simpl. 
-elim=>//=;intros. 
-move/eqP : H0=>Heq. subst=>//=. 
-asimpl. apply/H;eauto. asimpl.  apply (@muv_ren _ _ succn) in H0. 
-done. 
-Qed.
-
-Lemma muv_unf : forall g n, muv n g -> full_eunf g = EVar n. 
-Proof. 
-intros. rewrite /full_eunf. remember (emu_height g). 
-move : n0 g Heqn0 H.  
-elim=>//=. case=>//=. intros. f_equal=>//=. lia. 
-intros. 
-destruct g;try done. simpl in Heqn0.
-rewrite -iterS iterSr /=. rewrite H. done. 
-rewrite emu_height_subst. inv Heqn0=>//=. 
-case. 
-simpl. move/not_eguarded_muv=>Hm. simpl in H0. have : 0 = n.+1. 
-apply/muv_uniq;eauto. done. 
-done. 
-simpl in *. apply/muv_subst;eauto. simpl. done. 
-Qed.
-
-Lemma var_muv  : forall g n, g = EVar n -> muv n g. 
-Proof.
-case=>//=. intros. inv H. done. 
-Qed.*)
-
 Lemma unf_eguarded  : forall g n, eguarded n g  -> eunf g <> EVar n.  
 Proof. 
 case=>//=. intros. move => HH. inv HH. lia. 
@@ -200,14 +132,6 @@ move/H : H0. asimpl. move/(_ n0.+1). asimpl.
 move => HH. apply HH. apply/negP=> HH2. apply/negP. move : H1. move/negP/negP. eauto. 
 apply eguarded_ren2 in HH2. eauto. 
 Qed. 
-
-(*Lemma eguarded_subst2 : forall g n n0 sigma ,  eguarded n (g [e sigma]) ->  eguarded n0 g = false  -> eguarded n (sigma n0). 
-Proof. 
-elim=>//=;intros. have : n = n1 by lia. move=><-. done.
-move/H : H0. asimpl. move/(_ n0.+1). move/(_ H1). asimpl. 
-move/eguarded_ren2. done. 
-Qed. *)
-
 
 Lemma eguarded_eunf  : forall g n, eguarded n g -> eguarded n (eunf g).
 Proof. 
@@ -254,23 +178,11 @@ simpl in H. subst. simpl. destruct g;try done. simpl in H. move=> HH. inv HH. li
 rewrite iterSr.  apply H. apply/eguarded_eunf. done. 
 Qed.
 
-(*Lemma iter_unf_eguarded2  : forall n g, full_eunf g <> EVar n -> eguarded n g.
-Proof. intros. apply/eguarded_full_unf2. 
-destruct (full_eunf g) eqn:Heqn;try done. simpl. apply/negP=> HH. apply H. f_equal. lia.*) 
-
 Lemma eguarded_notn : forall e n, eguarded n e -> full_eunf e <> EVar n.
 Proof. 
 intros. apply eguarded_full_unf in H. destruct (full_eunf e);try done. simpl in H. move => HH. inv HH. lia. 
 Qed. 
 
-
-(*Lemma eguarded_subst3 : forall g n n0 sigma, eguarded n (sigma n0) -> muv n0 g -> muv n g[e sigma].
-Proof. simpl. 
-elim=>//=;intros. 
-move/eqP : H0=>Heq. subst=>//=. 
-asimpl. apply/H;eauto. asimpl.  apply (@muv_ren _ _ succn) in H0. 
-done. 
-Qed.*)
 
 Lemma eguarded_uniq : forall g n0 n1, eguarded n0 g = false -> eguarded n1 g = false -> n0 = n1.
 Proof. 
@@ -278,8 +190,6 @@ elim=>//=.
 intros. lia. 
 intros. suff : n0.+1 = n1.+1.  lia. apply/H=>//=. 
 Qed.
-
-
 
 Lemma eguarded_unfv : forall g n, eguarded n g = false -> full_eunf g = EVar n. 
 Proof. 
@@ -296,105 +206,6 @@ simpl in *. apply/negP=> HH. apply/negP. move/negP/negP : H0. eauto.
 eapply eguarded_subst2 in HH. eauto. asimpl. simpl. lia. 
 Qed.
 
-(*Lemma eguarded_not1 : forall n0 e n, iter n0 eunf e <> EVar n  -> eguarded n e.
-Proof.
-  elim;intros.  simpl in H . elim : n H . destruct e;try done.  simpl. apply/negP. move/eqP. move => HH. subst. eauto. 
-simpl. 
-apply eqP in HH. destruct 
-intros. destruct (eqVneq (full_eunf e) (EVar n)). done. exfalso. apply/negP. 
-move/negP/negP : H=>HH. apply/HH. 
-apply (negP H). H. apply/muv_unf. apply/not_eguarded_muv. lia. 
-Qed. 
-
-
-Lemma eguardedP : forall e n,  eguarded n e = (full_eunf e != EVar n).
-Proof. intros. apply/eq_iff. split. move/eguarded_not0. move/eqP.  lia. 
-intros. destruct (eguarded n e) eqn:Heqn. done. apply eguarded_not1 in Heqn. rewrite Heqn in H. 
-move : H. move/eqP. eauto. 
-Qed. 
-
-
-
-
-
-Lemma unf_eguarded  : forall g n, eunf g = EVar n -> eguarded n g = false. 
-Proof. 
-case=>//=. intros. inv H. lia. 
-intros. destruct e;try done.   move : H. 
-asimpl. destruct n0. done. asimpl. case. move=>->. 
-simpl. lia. 
-Qed.*)
-
-
-
-
-
-
-
-(*Lemma unf_muv  : forall g n, eunf g = EVar n -> muv n g. 
-Proof. 
-case=>//=. intros. inv H. done.
-intros. destruct e;try done.   move : H. 
-asimpl. destruct n0. done. asimpl. case. move=>->. 
-simpl. lia. 
-Qed.
-
-
-Lemma muv_ren2 : forall g n sigma, injective sigma ->  muv (sigma n) (g ⟨e sigma ⟩) -> muv n g.  
-Proof. 
-elim=>//=;intros. apply/eqP. apply/H. lia. 
-move : H1. asimpl. intros. apply/(@H _ (0 .: sigma >> succn)). 
-auto. asimpl. done.
-Qed.
-
-Lemma muv_subst2 : forall g n sigma, muv n (g [e sigma]) -> exists n0,  muv n0 g /\ muv n (sigma n0).
-Proof.
-elim=>//=;intros. 
-exists n. ssa. 
-apply H in H0.
-move : H0.  asimpl. 
-case. ssa. 
-destruct x;try done. 
-move : H1. asimpl. move/muv_ren2=>HH. 
-exists x. ssa. 
-Qed.
-
-
-
-Lemma muv_unf2 : forall g n,  muv n (eunf g) -> muv n g. 
-Proof. 
-case=>//=;intros.
-move : H. move/muv_subst2=>[] . 
-ssa. destruct x;try done. simpl in H0.
-rewrite (eqP H0). done. 
-Qed.
-
-Lemma muv_iter_unf2 : forall n0 g n,  muv n (iter n0 eunf g) -> muv n g. 
-Proof. 
-elim. case => //=. 
-intros. simpl in H0. apply/H.
-apply/muv_unf2. done. 
-Qed.
-
-Lemma muv_full_unf2 : forall g n,  muv n (full_eunf g) -> muv n g. 
-Proof. 
-intros. rewrite /full_eunf in H.  apply/muv_iter_unf2=>//=. eauto. 
-Qed.
-
-Lemma iter_unf_muv  : forall n0 n g, iter n0 eunf g = EVar n -> muv n g. 
-Proof. 
-elim;intros.
-simpl in H. subst. simpl. lia.
-simpl in H0. 
-apply unf_muv in H0. 
-apply/muv_iter_unf2. eauto. 
-Qed.*)
-
-(*Lemma eguarded_not_var : forall g n, eguarded n g -> muv n g = false. 
-Proof. 
-elim => //=;intros. lia. 
-auto. 
-Qed.*)
 
 Definition is_evar e := if e is EVar _ then true else false. 
 
@@ -456,36 +267,36 @@ Lemma ec_match : forall e, e = match e with | ECEnd => ECEnd | ECMsg d a u g0 =>
 Proof. case;auto. Qed.
 
 
-Definition e_to_c' (f : endpoint -> ecType)  g :=
+Definition etocoind' (f : endpoint -> ecType)  g :=
 match full_eunf g with 
 | EMsg d a u g0 =>  ECMsg d a u (f g0) 
 | EBranch d a gs => ECBranch d a (comap f (to_coseq gs))
 | _  => ECEnd
 end.
 
-CoFixpoint e_to_c g := e_to_c' e_to_c g. 
+CoFixpoint etocoind g := etocoind' etocoind g. 
 
-Lemma e_to_c'_eq g : e_to_c' e_to_c g =
+Lemma etocoind'_eq g : etocoind' etocoind g =
 match full_eunf g with 
-| EMsg d a u g0 =>  ECMsg d a u (e_to_c g0) 
-| EBranch d a gs => ECBranch d a (map e_to_c gs)
+| EMsg d a u g0 =>  ECMsg d a u (etocoind g0) 
+| EBranch d a gs => ECBranch d a (map etocoind gs)
 | _  => ECEnd
 end.
 Proof. 
-rewrite /e_to_c'. destruct (full_eunf g);try done. 
+rewrite /etocoind'. destruct (full_eunf g);try done. 
 f_equal. elim : l. simpl. rewrite !Utils.coeq comap_eq //=. 
 intros. rewrite Utils.coeq. rewrite Utils.comap_eqs /=. rewrite Utils.coeq.  f_equal. done. 
 Qed.
 
-Lemma e_to_c_eq g : e_to_c g = e_to_c' e_to_c g. 
+Lemma etocoind_eq g : etocoind g = etocoind' etocoind g. 
 Proof. 
-intros. rewrite /e_to_c'.  rewrite (ec_match (e_to_c g)). 
+intros. rewrite /etocoind'.  rewrite (ec_match (etocoind g)). 
 destruct g;try done;simpl. 
-rewrite /e_to_c'. 
+rewrite /etocoind'. 
 destruct (full_eunf (ERec g));try done. 
 Qed.
 
-Let e_to_cs_eqs := (e_to_c'_eq, e_to_c_eq). 
+Let etocoinds_eqs := (etocoind'_eq, etocoind_eq). 
 
 Lemma full_eunf_end  : full_eunf EEnd = EEnd.  
 Proof. done. Qed.
@@ -498,7 +309,7 @@ Proof. done. Qed.
 
 Let eunf_eqs := (full_eunf_end, full_eunf_msg, full_eunf_branch). 
 
-Let eqs := (Utils.comap_eqs,e_to_cs_eqs, eunf_eqs, Utils.coeq). 
+Let eqs := (Utils.comap_eqs,etocoinds_eqs, eunf_eqs, Utils.coeq). 
 
 Inductive EQ_gen  (R : ecType -> ecType -> Prop) : ecType -> ecType -> Prop := 
  | eq_end : EQ_gen R ECEnd ECEnd
@@ -515,179 +326,6 @@ move => es0 es1 d c. intros. constructor. apply/forall_gen_mon2. eauto. eauto. d
 Qed.
 
 Hint Resolve EQ_gen_mon : paco.
-
-(*
-
-
-
-(*Definition closed2 (A B : Type) (F0 F1 : (A -> B -> Prop) -> (A -> B -> Prop)) (R : A -> B -> Prop) := 
- F0 (F1 R) <2= (paco2 F1 R).  *)
-
-Variant SymF {A : Type} (R : A -> A -> Prop) : A -> A -> Prop  := 
- | symF_intro x0 x1: R x0 x1  -> SymF R x1 x0. 
-
-Hint Constructors SymF. 
-
-Variant Or {A B : Type} (R0 R1 : A -> B -> Prop) : A -> B -> Prop  := 
- | in_L x0 x1 : R0 x0 x1 -> Or R0 R1 x0 x1
- | in_R x0 x1: R1 x0 x1  -> Or R0 R1 x0 x1.
-Hint Constructors Or.
-
-
-Lemma  forall_gen_symFP 
-  : forall (A : Type) (P0 P1 : A -> A -> Prop) simC, SymF P0 <2= P1 ->
-    Or (SymF (paco2 (forall_gen P0) bot2)) <3= gupaco2 (forall_gen P1) (simC).
-Proof.
-  gcofix CIH. intros. destruct PR.  
-  inv H. punfold H1. inv H1. 
-  gstep.  constructor. 
-  gstep. constructor. eauto. pclearbot. gbase. eauto. 
-  gbase. done. 
-Qed.
-
-
-
-Lemma forall_gen_sym : forall (A : Type) (P0 P1  : A -> A -> Prop) , SymF P0 <2= P1 ->
-  SymF (paco2 (forall_gen P0) bot2)  <2= paco2 (forall_gen P1) bot2.
-Proof.
-intros. ginit. { eapply cpn2_wcompat. apply/forall_gen_mon.  } 
-guclo forall_gen_symFP.  
-Qed.
-
-Variant TransF {A : Type} (R : A -> A -> Prop) : A -> A -> Prop  := 
- | transF_intro x0 x1 x2: R x0 x1 -> R x1 x2  -> TransF R x0 x2. 
-
-Hint Constructors TransF. 
-
-
-Lemma  forall_gen_transFP 
-  : forall (A : Type) (P0 P1 : A -> A -> Prop) simC, TransF P0 <2= P1 -> 
-    Or (TransF (paco2 (forall_gen P0) bot2)) <3= gupaco2 (forall_gen P1) (simC).
-Proof.
-  gcofix CIH. intros. destruct PR.  
-  inv H. punfold H1. punfold H2. inv H1. inv H2. gstep. constructor. 
-  pclearbot. inv H2. gstep. constructor. eauto. 
-  pclearbot. gbase. eauto. 
-  gbase. done. 
-Qed.
-
-
-Lemma forall_gen_trans : forall (A : Type) (P0 P1  : A -> A -> Prop) , TransF P0 <2= P1 ->
-  TransF (paco2 (forall_gen P0) bot2)  <2= paco2 (forall_gen P1) bot2.
-Proof.
-intros. ginit. { eapply cpn2_wcompat. apply/forall_gen_mon.  } 
-guclo forall_gen_transFP.  
-Qed.*)
-
-
-
-
-(*Lemma sim_concat
-      s0 s1 t0 t1
-      (EQ0: sim s0 t0)
-      (EQ1: sim s1 t1)
-  :
-    @sim (concat s0 s1) (concat t0 t1)
-.
-Proof.
-  intros. ginit. { eapply cpn2_wcompat.  pmonauto. } guclo prefixC_spec.
-Qed.
-
-Lemma sim_concat_proper: Proper (sim ==> sim ==> sim) concat.
-Proof.
-  repeat intro. eapply sim_concat; eauto.
-Qed.
-
-
-Lemma forall_gen_sym : forall (A : Type) (r0 r1 : coseq A -> coseq A -> Prop)  (P0 P1 : A -> A -> Prop) ,
- symF P0 <2= P1 -> symF r0 <2= r1 -> symF (forall_gen P0 r0)  <2= paco2 (forall_gen P1) r1.
-Proof.
-intros. induction PR.  pc. pc. 
-Qed.*)
-
-
-(*Definition closed2 (A B : Type) (P : (A -> B -> Prop) -> (A -> B -> Prop) -> Prop) (F : (A -> B -> Prop) -> (A -> B -> Prop)) (R : A -> B -> Prop) := 
- P R R -> P (F R) (paco2 F R).  
-
-Definition sym_rel {A  : Type}  (F : (A -> A -> Prop) -> (A -> A -> Prop)) (R : A -> A -> Prop) :=
- forall a b, (F R) a b -> paco2 F R b a.*)
-
-
-
-(*Lemma forall_gen_sym : forall (A : Type) (r : coseq A -> coseq A -> Prop)  (P : A -> A -> Prop) , sym_rel P P ->
-  closed2  sym_rel (forall_gen P) r.
-Proof.
-rewrite /closed2 /sym_rel.  
-intros. move : a b H1. pcofix CIH. 
-intros. induction H2. pc. pc. 
-Qed.
-
-Definition trans_rel {A : Type}  (R0 R : A -> A -> Prop) := forall a b c, R0 a b -> R0 b c -> R a c.*)
-
-
-(*Definition transF (A : Type) (R : A -> A -> Prop) x0 x1 := exists x', R x0 x' /\ R x' x1. 
-
-Lemma forall_gen_trans : forall (A : Type) (r0 r1 : coseq A -> coseq A -> Prop)  (P0 P1 : A -> A -> Prop) ,
- transF P0 <2= P1 -> transF r0 <2= r1 -> transF (forall_gen P0 r0)  <2= paco2 (forall_gen P1) r1.
-Proof.
-rewrite /transF. intros. destruct PR,H1. induction H1. inv H2. pc. 
-inv H2. subst. pc. apply/H. exists e1. ssa. right.  apply/H0. exists es1. ssa. 
-Qed.*)
-
-(*Lemma forall_gen_trans : forall (A : Type) (r : coseq A -> coseq A -> Prop)  (P : A -> A -> Prop) , trans_rel P P ->
-  closed2  trans_rel (forall_gen P) r.
-Proof.
-rewrite /closed2 /trans_rel.  
-intros. move : a b H1 H2. pcofix CIH. 
-intros. induction H2. inv H3. pc. inv H3. 
-subst. pc. eauto. eauto. 
-Qed.*)
-
-
-
-(*Lemma forall_gen_sym : forall (A : Type) (r : coseq A -> coseq A -> Prop)  (P : A -> A -> Prop) , 
-  @closed2 (coseq A) (coseq A) (@sym_rel (coseq A)) (forall_gen P) r. 
-
-
-(forall x y, r x y -> r y x) ->
- (forall x y, P x y -> P y x) -> (forall_gen P) r g0 g1 ->  g1 <<(r) (forall_gen P)  >>  g0. 
-
-Lemma forall_gen_sm
-Check (@closed2 _ _ sym_rel EQ_gen bot2).
-
-
-Lemma forall_gen_sym : forall (A : Type) g0 g1 (r : coseq A -> coseq A -> Prop)  (P : A -> A -> Prop) , (forall x y, r x y -> r y x) ->
- (forall x y, P x y -> P y x) -> (forall_gen P) r g0 g1 ->  g1 <<(r) (forall_gen P)  >>  g0. 
-Proof. 
-intros. move : g0 g1 H1. pcofix CIH. 
-intros. induction H2. pc. pc. 
-Qed.
-
-Lemma forall_gen_trans : forall (A : Type) g0 g1 g2 (r : coseq A -> coseq A -> Prop)  (P0 P1 P2 : A -> A -> Prop) , (forall x y z, x <<(bot2) (forall_gen P0) >>  y -> r y z -> r x z) -> (forall x y z, P0 x y -> P1 y z -> P2 x z) -> 
- g0 <<(bot2) (forall_gen P0) >> g1 -> (forall_gen P1) r g1 g2 ->  g0 <<(r) (forall_gen P2)  >>  g2. 
-Proof. 
-intros. move : g0 g1 g2 H1 H2. pcofix CIH. 
-intros. uis H2. uis H3.
-uis H3. eauto. pclearbot.   inv H9. right.  apply /CIH. apply H4. done. 
-right. eauto. 
-Qed.*)
-
-(*Lemma forall_gen_sym : forall (A : Type) g0 g1 (r : coseq A -> coseq A -> Prop)  (P : A -> A -> Prop) , (forall x y, r x y -> r y x) -> (forall x y, P x y -> P y x) -> g0 <<(r) (forall_gen P)  >>  g1 ->  g1 <<(r) (forall_gen P)  >>  g0. 
-Proof. 
-intros. move : g0 g1 H1. pcofix CIH. 
-intros. uis H2. inv H3.  
-right. apply/CIH. done.
-auto.  
-Qed.*)
-
-(*Lemma forall_gen_trans : forall (A : Type) g0 g1 g2 (r : coseq A -> coseq A -> Prop)  (P0 P1 P2 : A -> A -> Prop) , (forall x y z, x <<(bot2) (forall_gen P0) >>  y -> r y z -> r x z) -> (forall x y z, P0 x y -> P1 y z -> P2 x z) -> 
- g0 <<(bot2) (forall_gen P0) >> g1 ->  g1 <<(r) (forall_gen P1)  >>  g2 ->  g0 <<(r) (forall_gen P2)  >>  g2. 
-Proof. 
-intros. move : g0 g1 g2 H1 H2. pcofix CIH. 
-intros. uis H2. uis H3.
-uis H3. eauto. pclearbot.   inv H9. right.  apply /CIH. apply H4. done. 
-right. eauto. 
-Qed.*)
 
 
 Lemma EQ_refl : forall g r,  g <<(r) EQ_gen  >>  g. 
@@ -729,178 +367,6 @@ right. apply/CIH2.  pclearbot. eauto. pclearbot. eauto.
 Qed.
 
 
-(*Lemma sym_forall : forall (A : Type) (P : A -> A -> Prop) (R : coseq A -> coseq A -> Prop), forall_gen P R <2= symF (forall_gen (symF P) (symF R)).
-Proof. 
-intros. rewrite /symF.  induction PR. constructor. 
-constructor. done. done. 
-Qed.*)
-
-(*Lemma  EQ_gen_symFP 
-  : forall simC,
-    Or (SymF (paco2 EQ_gen bot2)) <3= gupaco2 EQ_gen (simC).
-Proof.
-  gcofix CIH. intros. destruct PR.  
-  inv H. punfold H0. inv H0. 
-  gstep.  constructor. 
-  gstep. constructor. pclearbot. gfinal. eauto.  
-  gstep. constructor. apply/forall_gen_sym. intros.
-  2 : {  constructor. eauto. } 
-  inv PR. pclearbot. gbase. apply/CIH. left. constructor. done. 
-  gbase. done. 
-Qed.
-
-Lemma EQ_gen_sym : (SymF (paco2 EQ_gen bot2)) <2= paco2 EQ_gen bot2. 
-Proof.
-intros. ginit. { eapply cpn2_wcompat. apply EQ_gen_mon.  } 
-guclo EQ_gen_symFP.  
-Qed.
-
-
-Lemma  EQ_gen_transFP 
-  : forall simC,
-    Or (TransF (paco2 EQ_gen bot2)) <3= gupaco2 EQ_gen (simC).
-Proof.
-  gcofix CIH. intros. destruct PR.  
-  inv H. punfold H0. punfold H1. inv H0. inv H1. 
-  gstep.  constructor. pclearbot.  inv H1.
-  gstep. constructor. pclearbot. gfinal. eauto.  
-  gstep. inv H1. constructor. apply/forall_gen_trans. intros.
-  2 : {  econstructor. eauto. done. } 
-  inv PR. pclearbot. gbase. apply/CIH. left. eauto. 
-  gbase. done. 
-Qed.*)
-
-
-
-(*CoFixpoint comap (A B : Type)  (f : A -> B)  (aa : coseq A):= 
-match aa with 
-| conil => conil 
-| cocons a aa' => cocons (f a) (comap f aa')
-end.
-
-
-CoFixpoint e_to_ec e :=
-let cofix e_to_ecs  aa := 
-match aa with 
-| nil => conil 
-| cons a aa' => cocons (e_to_ec a) (e_to_ecs aa')
-end in 
-match full_eunf e  with 
-| EMsg d c u e0 =>  ECMsg d c u (e_to_ec e0) 
-| EBranch d c es => ECBranch d c (e_to_ecs es)
-| _  => ECEnd
-end.
-
-CoFixpoint e_to_ecs  aa := 
-match aa with 
-| nil => conil 
-| cons a aa' => cocons (e_to_ec a) (e_to_ecs aa')
-end.
-
-Lemma e_to_ecs_nil : e_to_ecs nil = conil. 
-Proof. rewrite (coseq_match (e_to_ecs _)) //=. 
-Qed.
-
-Lemma e_to_ecs_cons a b : e_to_ecs (a::b) = cocons (e_to_ec a) (e_to_ecs b). 
-Proof. 
-rewrite (coseq_match (e_to_ecs _)) /=. done. 
-Qed.
-
-
-
-Lemma comap_nil : comap e_to_ec nil = nil. 
-Proof.
-rewrite (coseq_match (comap _ _)) /=.  coseq_tac. done. 
-Qed. 
-
-
-Lemma comap_cons : forall (A B : Type) (a : A) l (f : A -> B), comap f (cocons a l) = cocons (f a) (comap f l). 
-Proof.
-intros. rewrite (coseq_match (comap _ _)) /=. done. 
-Qed.
-
-
-
-Let coeq := (e_to_ecs_nil, e_to_ecs_cons,Utils.coeq). 
-
-
-Lemma cofix_comap  : forall aa, ((cofix comap  aa := 
-match aa with 
-| nil  => conil 
-| cons a aa' => cocons (e_to_ec a) (comap aa')
-end) aa) = e_to_ecs aa. 
-Proof. 
-elim. done. intros. rewrite coeq /=. 
-rewrite (coseq_match  (_ (_::_))). f_equal.  
-Qed.
-
-
-
-
-Lemma e_to_ec_eq : forall e, e_to_ec e =
-(match full_eunf e  with 
-| EMsg d c u g0 =>  ECMsg d c u (e_to_ec g0) 
-| EBranch d c es => ECBranch d c (e_to_ecs es)
-| _  => ECEnd
-end). 
-Proof.
-move => e. rewrite (ec_match (e_to_ec e)).
-rewrite /e_to_ec. destruct (full_eunf e);try done. 
-Qed.*)
-
-(*Lemma e_to_ec_branch : forall e d c es, full_eunf e = EBranch d c es -> (e_to_ec e) =(E)= ECBranch d c (comap e_to_ec (to_coseq es)).
-Proof.  
-intros. 
-rewrite e_to_ec_eq. *)
-(*Define equality on streams*)
-
-(*CoFixpoint e_to_ecs (es : seq endpoint) : coseq ecType := 
- match es with 
- | nil => conil
- | e' :: es' => cocons (e_to_ec e') (e_to_ecs es')
- end.*)
-
-
-
-
-
-
-
-
-
-(*Lemma e_to_ecs_eq : forall es, e_to_ecs es = 
- match es with 
- | nil => conil 
- | g' :: gs' => cocons (e_to_ec g') (e_to_ecs gs')
- end. 
-Proof. 
-move => es. rewrite (coseq_match (e_to_ecs es)). destruct es. done. simpl. f_equal. 
-Qed. *)
-
-
-
-
-
-(*Inductive forallIC_gen {A B : Type} (P : A -> B -> Prop)  (R : seq A -> coseq B -> Prop)  : seq A -> coseq B -> Prop :=
-| FEEIC_nil : forallIC_gen P R nil conil
-| FEEIC_cons e0 e1 es0 es1 : P e0 e1 -> R es0 es1 -> forallIC_gen P R (cons e0 es0) (cocons e1 es1).
-Lemma forallIC_gen_mon (A B : Type) (P : A -> B -> Prop)  : monotone2 (forallIC_gen P). 
-Proof. 
-move => x y. intros. induction IN. constructor. constructor. done. auto. 
-Qed. 
-
-Hint Resolve forallIC_gen_mon : paco. 
-
-Definition ForallIC {A B : Type} (P : A -> B -> Prop)  es0 es1 := paco2 (forallIC_gen P) bot2 es0 es1. 
-
-Lemma ForallIC_mon : forall (A B : Type) (P0 P1: A -> B -> Prop) es0 es1, (forall x0 x1, P0 x0 x1 -> P1  x0 x1) -> ForallIC P0 es0 es1 -> ForallIC P1 es0 es1. 
-Proof.
-move => A B P0 P1.
-pcofix CIH. 
-intros. pfold. punfold H1. inversion H1. subst. constructor. subst. 
-constructor. auto. right. apply/CIH. auto. pclearbot. eauto. 
-Qed.*)
-
 Inductive Unravele_gen (R : endpoint -> ecType  -> Prop) : endpoint -> ecType  -> Prop :=
  | Unravele_gen_msg e0 ec d c u : R e0 ec -> Unravele_gen R (EMsg d c u e0) (ECMsg d c u ec)
  | Unravele_gen_branch (es : seq endpoint) (ecs : seq ecType) d c : size es = size ecs -> Forall (R_pair R) (zip es ecs)   -> Unravele_gen R (EBranch d c es) (ECBranch d c ecs)
@@ -918,7 +384,7 @@ Qed.
 
 Hint Resolve Unravele_gen_mon : paco. 
 
-Definition Unravele e0 e1 := paco2 Unravele_gen bot2 e0 e1.
+Notation Unravele e0 e1 := (paco2 Unravele_gen bot2 e0 e1).
 
 
 
@@ -936,24 +402,15 @@ Qed.
 
 Hint Resolve Unravele2_gen_mon. 
 
-Lemma e_to_c_full_eunf : forall e, e_to_c e = e_to_c (full_eunf e). 
+Notation UnfUnravele := (ApplyF full_eunf ssrfun.id). 
+Notation Unravele2 e0 e1 := (paco2  (UnfUnravele \o Unravele2_gen) bot2 e0 e1).
+
+Lemma etocoind_full_eunf : forall e, etocoind e = etocoind (full_eunf e). 
 Proof. 
 intros. rewrite !eqs full_eunf_idemp //=.
 Qed.
 
-Notation UnfUnravele := (ApplyF full_eunf ssrfun.id). 
 
-
-
-
-Lemma Unravele_unf  : forall (F : (endpoint -> ecType -> Prop) -> (endpoint -> ecType -> Prop)) a b r, monotone2 F ->  paco2 (UnfUnravele \o F) r  a b <->  paco2 (UnfUnravele \o F) r  (full_eunf a) b.
-Proof. 
-intros. 
-split. 
-intros. punfold H0. inv H0. pfold. constructor. rewrite full_eunf_idemp. done. 
-intros. punfold H0.  pfold. rewrite /comp. rewrite /comp in H0. inv H0. 
-rewrite full_eunf_idemp in H1. constructor. done. 
-Qed.
 
 Lemma Unravele_eunf4 :  forall e ec (R: endpoint -> ecType -> Prop), paco2 Unravele_gen R (eunf e) ec -> paco2 Unravele_gen R e ec.
 Proof.
@@ -971,7 +428,7 @@ intros. rewrite /full_eunf in H. apply/Unravele_eunf5.  eauto.
 Qed.
 
 
-Lemma Unravele_iff : forall e ec, e << Unravele_gen >> ec <->  e << (UnfUnravele \o Unravele2_gen)  >> ec. 
+Lemma Unravele_iff : forall e ec, Unravele e ec <-> Unravele2 e ec.
 Proof.
 Proof. intros. split. 
 move : e ec. pcofix CIH. 
@@ -979,13 +436,6 @@ intros. punfold H0.  induction H0. pclearbot. pfold.
 constructor. rewrite /full_eunf /=.  constructor. eauto. 
 pfold. constructor. rewrite /full_eunf /=. constructor. done. 
 induction H0;auto. constructor. pclearbot. eauto. eauto.  
-(*pclearbot. 
-brewr
-move : gs gcs H. elim;intros. 
-rewrite coeq in H. rewrite coeq. 
-uis H. 
-rewrite coeq in H0. rewrite coeq. uis H0. eauto.  
-left. apply/H. done. *)
 pfold. constructor. rewrite full_eunf_subst. 
 punfold IHUnravele_gen. inv IHUnravele_gen. done.
 pfold. constructor. rewrite /full_eunf. constructor.
@@ -1000,28 +450,22 @@ Qed.
 
 
 
-
-Lemma Unravele_uniq : forall e ec0 ec1, e << Unravele_gen >> ec0 ->  e  << Unravele_gen >> ec1 -> ec0 << EQ_gen >> ec1. 
+Lemma Unravele_uniq : forall e ec0 ec1, Unravele2 e ec0 ->  Unravele2 e ec1 -> ec0 << EQ_gen >> ec1. 
 Proof. 
-pcofix CIH. 
-move => e ec0 ec1 HH. punfold HH. induction HH. pclearbot.
-move => HH2. punfold HH2. inversion HH2;subst.  
-pfold. constructor. right. apply/CIH. eauto. pclearbot. done. 
-move => HH2. punfold HH2. inversion HH2;subst. 
-pfold. constructor. clear HH2. 
-eapply coerce_forall2.  lia.
-
-move : es ecs ecs0 H H0 H5 H6. 
-elim. case;last done.  case;last done.  simpl. auto. 
-move => a0 l IH. case;first done. move => a1 l0. case;first done. 
-intros. simpl in *. inv H. inv H5. inv H0.  inv H6. pclearbot. simpl in *.
-constructor. rewrite /R_pair /=. eauto. eauto. 
-move => HH2. punfold HH2. inversion HH2. subst. 
- apply/IHHH. pfold. done. 
-move => HH2. punfold HH2. inversion HH2. pfold. constructor. 
+pcofix CIH. intros. punfold H0. punfold H1. inv H0. inv H1. inv H;pclearbot.
+rewrite -H3 in H2. inv H2;pc.  inv H10;try done. right. apply/CIH. eauto. eauto.
+rewrite -H3 in H2. inv H2. pfold. con. apply coerce_forall2. lia. 
+clear H0 H1 H2 H3 H. 
+elim : es ecs ecs0 H4 H10 H5 H11.
+case=>//=. case=>//=.
+move => a l  IH [] //=. move => a0 l0 [] //=. move => a1 l1. intros. inv H4. inv H10.  inv H5.  inv H11.
+pclearbot. ssa. 
+con;eauto. 
+rewrite -H4 in H2. inv H2. 
+pfold. con. 
 Qed.
 
-Lemma Unravele_eq : forall g gc0 gc1, gc0 << EQ_gen >> gc1 ->  g << (ApplyF full_eunf ssrfun.id \o Unravele2_gen) >> gc0 ->  g  << (ApplyF full_eunf ssrfun.id \o  Unravele2_gen) >> gc1.
+Lemma Unravele_eq : forall g gc0 gc1, gc0 << EQ_gen >> gc1 ->  Unravele2 g gc0 ->  Unravele2 g gc1.
 Proof.
 pcofix CIH. 
 intros. punfold H1. pfold.   constructor. inv H1. induction H;pclearbot. uis H0.
@@ -1039,33 +483,27 @@ uis H0. constructor.
 Qed.
 
 
-Lemma e_to_c_rec e : (e_to_c (ERec e)) = e_to_c (e [e ERec e .: EVar]). 
+Lemma etocoind_rec e : (etocoind (ERec e)) = etocoind (e [e ERec e .: EVar]). 
 Proof.
 rewrite 4!eqs full_eunf_subst //=.  
 Qed.
 
 
 (*Later perhaps do it with gpaco*)
-Lemma unravele_exist : forall e,  e << Unravele_gen >> (e_to_c e) <-> exists ec, e << Unravele_gen >>  ec.
+Lemma unravele_exist : forall e,  Unravele2 e (etocoind e) <-> exists ec, Unravele2 e  ec.
 Proof. 
 intros. split. 
-intros. exists (e_to_c e).  done.
+intros. exists (etocoind e).  done.
 case. move : e. 
 intros. 
 move : x e p. pcofix CIH. 
-move => x e Hu. punfold Hu. induction Hu.
-pfold. rewrite 3!eqs. constructor. pclearbot.  eauto. 
-rewrite 3!eqs. pfold. constructor. 
-rewrite size_map //=.
-elim : es ecs H H0. case. simpl. auto. done. 
-move => a0 l IH []. done. simpl in *. ssa. inv H0.  
-simpl in *. pclearbot. constructor; eauto. 
-pfold. constructor. 
-rewrite e_to_c_rec. 
-punfold IHHu. 
-rewrite !eqs. pc. 
-Qed.
-
+move => x e Hu. punfold Hu. inv Hu. 
+pfold. con. rewrite etocoind_full_eunf.
+ inv H;rewrite 3!eqs;try con;eauto;pclearbot. eauto. rewrite size_map. done. 
+clear H Hu H0. 
+elim :es ecs H1 H2. case;try done.  ssa. move => a l IH [] //=.  ssa. 
+con. inv H2.  pclearbot. ssa. right. eauto. inv H2. ssa. eapply IH. eauto. done. 
+Qed. 
 
 Fixpoint enum e :=
 e::
@@ -1265,8 +703,6 @@ Hint Resolve EQ2_gen_mon : paco.
 Notation EQ2 := (fun e0 e1 => paco2 ((ApplyF full_eunf full_eunf) \o EQ2_gen) bot2 e0 e1).
 
 
-Notation Unravele2 := (fun e ec =>  paco2 (UnfUnravele \o Unravele2_gen) bot2 e ec).
-
 Ltac pc := pclearbot.
 
 Lemma EQ2_spec1 : forall e0 e1 ec0 ec1, Unravele2 e0 ec0 -> Unravele2 e1 ec1 ->  EQ2 e0 e1 -> paco2 EQ_gen bot2 ec0 ec1. 
@@ -1329,28 +765,11 @@ Proof.
 intros. punfold H. inv H. pfold. con. rewrite full_eunf_idemp. done. 
 Qed.
 
-Inductive Rollinge2_gen (R : endpoint ->  Prop) : endpoint   -> Prop :=
- | role3_gen_msg e0 c d u :  R e0 -> Rollinge2_gen R  (EMsg d c u e0) 
- | role3_gen_branch c (es : seq endpoint)  d :  Forall R es -> Rollinge2_gen R (EBranch d c es) 
- | role4_gen_end :   Rollinge2_gen R EEnd
- | role4_gen_rec e : Rollinge2_gen R (e [e ERec e .: EVar]) ->  Rollinge2_gen R (ERec e).
-
-Lemma Rollinge2_gen_mon : monotone1 Rollinge2_gen. 
-Proof. move => x0 x1. intros. induction IN;try done. con;eauto. 
-con;eauto. apply/List.Forall_forall. intros. eauto. 
-move/List.Forall_forall : H. eauto. con. con. eauto. 
-Qed. 
-
-
-Hint Resolve Rollinge2_gen_mon : paco. 
-
-
 
 Inductive Rollinge_gen (R : endpoint ->  Prop) : endpoint   -> Prop :=
  | role2_gen_msg e0 c d u :  R e0 -> Rollinge_gen R  (EMsg d c u e0) 
  | role2_gen_branch c (es : seq endpoint)  d :  Forall R es -> Rollinge_gen R (EBranch d c es) 
  | role2_gen_end :   Rollinge_gen R EEnd.
-(* | role2_gen_rec e : Rollinge_gen R (e [e ERec e .: EVar]) ->  Rollinge_gen R (ERec e).*)
 
 Lemma Rollinge_gen_mon : monotone1 Rollinge_gen. 
 Proof. move => x0 x1. intros. induction IN;try done. con;eauto. 
@@ -1361,53 +780,6 @@ Qed.
 
 Hint Resolve Rollinge_gen_mon : paco. 
 Notation Rollinge := (paco1 (ApplyF1 full_eunf \o Rollinge_gen) bot1).  
-
-
-Lemma rollinge_eunf4 :  forall e (R: endpoint -> Prop), Rollinge2_gen R (eunf e) -> Rollinge2_gen R e.
-Proof.
-intros.  destruct e;try done. con. simpl in H. done. 
-Qed.
-
-Lemma rollinge_eunf5 :  forall n e (R: endpoint -> Prop), Rollinge2_gen R (iter n eunf e)  -> Rollinge2_gen R e.
-Proof.
-elim. done. intros. simpl in H0. apply rollinge_eunf4 in H0. auto. 
-Qed.
-
-Lemma rollinge_eunf6 :  forall e (R: endpoint -> Prop), Rollinge2_gen R (full_eunf e)  -> Rollinge2_gen R e.
-Proof. 
-intros. rewrite /full_eunf in H. apply/rollinge_eunf5.  eauto. 
-Qed.
-
-
-(*Lemma rollinge_eunf7 :  forall e (R: endpoint -> Prop), Rollinge2_gen R e -> Rollinge2_gen R (eunf e).
-Proof.
-intros.  destruct e;try done. simpl. inv H. done. 
-Qed.
-
-Lemma rollinge_eunf8 :  forall n e (R: endpoint -> Prop), Rollinge2_gen R e -> Rollinge2_gen R (iter n eunf e).  
-Proof.
-elim. done. intros. simpl in H0. apply rollinge_eunf7 in H0. rewrite iterSr.  auto. 
-Qed.
-
-Lemma rollinge_eunf9 :  forall e (R: endpoint -> Prop), Rollinge2_gen R e  -> Rollinge2_gen R (full_eunf e).
-Proof. 
-intros. rewrite /full_eunf in H. apply/rollinge_eunf8.  eauto. 
-Qed.
-*)
-
-Lemma FEQP : forall R x, (ApplyF1 full_eunf \o Rollinge_gen) R x <-> Rollinge2_gen R x. 
-Proof. 
-intros. split. case. intros. apply/rollinge_eunf6. inv r;eauto. con. done. 
-con. done. con. 
-intros. con. 
-induction H. con. done. con. done. con. 
-rewrite full_eunf_subst. done. 
-Qed. 
-
-
-
-
-
 
 Lemma EQ2_tree : forall e0 e1, EQ2 e0 e1 -> Rollinge e0.
 Proof. 
@@ -1425,12 +797,12 @@ con. clear H1 H2. elim : es0 es1 H3 H4. case. done. done.
 move => a l IH [] //=. intros. inv H3. inv H4. pc. simpl in *. con; eauto. 
 Qed. 
 
-Lemma Rolling_Unravele : forall g ,  Rollinge g -> paco2 (UnfUnravele \o Unravele2_gen) bot2 g (e_to_c g).
+Lemma Rolling_Unravele : forall g ,  Rollinge g -> Unravele2 g (etocoind g).
 Proof. 
 pcofix CIH. intros. punfold H0. inv H0. pfold.
-rewrite e_to_c_full_eunf.  con. 
+rewrite etocoind_full_eunf.  con. 
 inv H;eauto;pclearbot;rewrite !eqs.  
-rewrite -e_to_c'_eq -e_to_c_eq. con. eauto. 
+rewrite -etocoind'_eq -etocoind_eq. con. eauto. 
 con. rewrite size_map //=. 
 clear H H1 H0. elim : es H2. simpl.  auto. 
 simpl. intros. inv H2. pclearbot. con. eauto. eauto. 
@@ -1440,7 +812,7 @@ Qed.
 
 Theorem EQ2_spec : forall e0 e1, EQ2 e0 e1 <-> exists ec0 ec1, Unravele2 e0 ec0 /\ Unravele2 e1 ec1 /\ paco2 EQ_gen bot2 ec0 ec1. 
 Proof. 
-intros. split. intros. exists (e_to_c e0). exists (e_to_c e1). ssa. 
+intros. split. intros. exists (etocoind e0). exists (etocoind e1). ssa. 
 apply/Rolling_Unravele/EQ2_tree. eauto. 
 apply/Rolling_Unravele/EQ2_tree2. eauto. apply/EQ2_spec1.
 apply/Rolling_Unravele. apply/EQ2_tree. eauto. 
