theories/Projection.v
@@ -9,23 +9,28 @@ Unset Printing Implicit Defensive.
 Let eqs := ProjectSpec.eqs. 
 
 
-Fixpoint projectT p g := 
+Fixpoint trans p g := 
 match g with 
-| GMsg a u g0 => if comp_dir p a is Some d then  EMsg d (action_ch a) u (projectT p g0) else projectT p g0
-| GBranch a gs => if comp_dir p a is Some d then EBranch d (action_ch a) (map (projectT p) gs) 
-                                           else head EEnd (map (projectT p) gs)
-| GRec g0 => let e := projectT p g0 in if eguarded 0 e then ERec e else EEnd
+| GMsg a u g0 => if comp_dir p a is Some d then  EMsg d (action_ch a) u (trans p g0) else trans p g0
+| GBranch a gs => if comp_dir p a is Some d then EBranch d (action_ch a) (map (trans p) gs) 
+                                           else head EEnd (map (trans p) gs)
+| GRec g0 => let e := trans p g0 in if eguarded 0 e then ERec e else EEnd
 | GVar n => EVar n
 | GEnd => EEnd 
 end. 
 
 Definition project (g : gType) (p : ptcp) : option endpoint := 
-let e := projectT p g in if projectb g p e then Some e else None. 
+let e := trans p g in if projectb g p e then Some e else None. 
 
-Lemma project_sound : forall g p e, project g p = Some e -> Project g p e. 
+Lemma project_sound_aux : forall g p e, project g p = Some e -> Project g p e. 
 Proof. 
 intros. rewrite /project in H. move : H. case_if. case. 
 move=><-.  apply/projectb_iff. done. done.
+Qed.
+
+Lemma project_sound : forall g p e, project g p = Some e -> exists gc ec, Unravelg2 g gc /\ Unravele2 e ec /\ CProject gc p ec. 
+Proof. 
+intros. move/project_sound_aux : H. move/ICProject_iff=>//=. 
 Qed.
 
 (*The rest of this file shows completeness*)
@@ -39,10 +44,10 @@ match e with
 end.  
 
 
-(*property for projectT recursively defined, so shown by induction on g satisfying muve assuming inp both recursively defined,
+(*property for trans recursively defined, so shown by induction on g satisfying muve assuming inp both recursively defined,
  part_of 2 -> inp -> part_of3 ->  part_of2 
  *)
-Lemma inp_muve : forall p g, ~~ inp p g  -> muve (projectT p g). 
+Lemma inp_muve : forall p g, ~~ inp p g  -> muve (trans p g). 
 Proof. 
 move => p. elim;intros. done. done. 
 simpl. 
@@ -81,7 +86,7 @@ match g with
 | ERec g0 => (eguarded 0 g0) && (econtractive2 g0)
 end. 
 
-Lemma project_econtractive2 : forall p g, econtractive2 (projectT p g). 
+Lemma project_econtractive2 : forall p g, econtractive2 (trans p g). 
 Proof. 
 move => p. elim;intros=>//=.  
 case_if. ssa.   done. 
@@ -112,6 +117,8 @@ Fixpoint gType_fv2 e :=
   | GBranch _ gs => flatten (map gType_fv2 gs)
   | GRec g0 => map predn (filter (fun n => n != 0) (gType_fv2 g0))
   end.
+
+Definition gclosed g := forall n, n \notin gType_fv2 g.
 
 Lemma gType_fv2_ren : forall g sigma, (gType_fv2 g ⟨g sigma⟩) = map sigma (gType_fv2 g). 
 Proof. 
@@ -186,6 +193,8 @@ Fixpoint endpoint_fv2 e :=
   | ERec g0 => map predn (filter (fun n => n != 0) (endpoint_fv2 g0))
   end.
 
+Definition eclosed e := forall n, n \notin endpoint_fv2 e.
+
 Lemma endpoint_fv2_ren : forall g sigma, (endpoint_fv2 g ⟨e sigma⟩) = map sigma (endpoint_fv2 g). 
 Proof. 
 elim;rewrite //=;intros. 
@@ -249,7 +258,7 @@ Qed.
 
 
 
-Lemma fv_proj : forall g p n, n \in endpoint_fv2 (projectT p g) -> n \in gType_fv2 g. 
+Lemma fv_proj : forall g p n, n \in endpoint_fv2 (trans p g) -> n \in gType_fv2 g. 
 Proof. 
 elim=>//=;intros. 
 move : H0. case_if. simpl. move/mapP=>[] . intros. subst. rewrite mem_filter in p0. ssa. 
@@ -265,19 +274,19 @@ destruct l;try done.
 ssa. rewrite mem_cat. apply/orP. left. apply/H=>//=. eauto. 
 Qed.
 
-Lemma fv_proj_not : forall g p n, n \notin gType_fv2 g -> n \notin endpoint_fv2 (projectT p g).
+Lemma fv_proj_not : forall g p n, n \notin gType_fv2 g -> n \notin endpoint_fv2 (trans p g).
 Proof. 
 intros. apply/negP. move => HH. apply/negP. apply/H. apply/fv_proj. eauto. 
 Qed. 
 
 
 
-Lemma EQ_end_aux : forall p g, Rolling g -> ~~ inp p g -> full_eunf (projectT p g) = EEnd.  
+Lemma EQ_end_aux : forall p g, Rolling g -> ~~ inp p g -> full_eunf (trans p g) = EEnd.  
 Proof. 
 intros. apply inp_muve in H0. 
 move : (@project_econtractive2 p g)=>HH. 
-have : leaf (full_eunf (projectT p g)).  apply/muve_leaf. eauto. done. 
-intros. destruct (full_eunf (projectT p g)) eqn:Heqn;try done. Check Rolling_no_fv.
+have : leaf (full_eunf (trans p g)).  apply/muve_leaf. eauto. done. 
+intros. destruct (full_eunf (trans p g)) eqn:Heqn;try done. Check Rolling_no_fv.
 move/Rolling_no_fv : H. move/(_ n). move/fv_proj_not.
 move/(_ p). 
 rewrite endpoint_fv2_full_eunf Heqn /= inE.  lia. 
@@ -288,7 +297,7 @@ Qed.
 
 
 Theorem EQ_end : forall p g, ~ part_of2 p g -> Rolling g ->
-  EEnd << (ApplyF full_eunf full_eunf \o EQ2_gen) >> (projectT p g).
+  EEnd << (ApplyF full_eunf full_eunf \o EQ2_gen) >> (trans p g).
 Proof. 
 intros. apply/EQ2_eunf. erewrite  EQ_end_aux. pfold. con. con. done. apply/negP. move => HH. apply H. 
 apply/inp_iff. done. 
@@ -296,14 +305,14 @@ Qed.
 
 
 (*Switch from eguarded because we have a comm lemma on renaimg without strong assumption prevents doing the same in project_subst*)
-Lemma project_ren : forall p g sigma, injective sigma ->  projectT p g ⟨g sigma ⟩ = (projectT p g) ⟨e sigma ⟩. 
+Lemma project_ren : forall p g sigma, injective sigma ->  trans p g ⟨g sigma ⟩ = (trans p g) ⟨e sigma ⟩. 
 Proof. 
 move => p. elim;intros;asimpl.  
 simpl. done. 
 done. 
 simpl. rewrite H. 
 have : injective (0 .: sigma >> succn). auto. move/eguarded_ren_iff. 
-move/(_ (projectT p g) 0)=>/=. move/eq_iff=><-. case_if=>//=. auto. 
+move/(_ (trans p g) 0)=>/=. move/eq_iff=><-. case_if=>//=. auto. 
 asimpl. simpl. destruct (comp_dir _ _);try done. simpl. rewrite H. done. done. 
 auto. simpl. destruct (comp_dir _ _);try done. simpl. rewrite -!map_comp. 
 f_equal. apply/eq_in_map=> x xIn. simpl. auto. 
@@ -329,20 +338,20 @@ rewrite !inE in H. lia.
 apply H. move : H0. intros. apply/negP=>HH'. apply/negP. apply H0. apply/mapP. exists v.+1. rewrite mem_filter. ssa. done. 
 Qed.
  
-Lemma project_subst  : forall p g sigma, projectT p g [g sigma ] = (projectT p g) [e sigma >> projectT p ]. 
+Lemma project_subst  : forall p g sigma, trans p g [g sigma ] = (trans p g) [e sigma >> trans p ]. 
 Proof. 
 move => p. elim;intros;asimpl.  
 simpl. done. 
 done. 
 simpl.  rewrite H. asimpl. simpl. 
 symmetry.  case_if. 
-have :  eguarded 0 (projectT p g) [eEVar 0 .: sigma >> (⟨g ↑ ⟩ >> projectT p)]. apply/eguarded_sig2. 
+have :  eguarded 0 (trans p g) [eEVar 0 .: sigma >> (⟨g ↑ ⟩ >> trans p)]. apply/eguarded_sig2. 
 instantiate (1 := EVar). asimpl. done. case. done. simpl. intros. asimpl. rewrite project_ren //=. 
 apply/eguarded_fv. rewrite endpoint_fv2_ren. 
 apply/negP=>HH. move/mapP : HH. case. ssa. 
 move=>->. simpl. f_equal. asimpl. simpl. f_equal. fext. case.  done. move => n. simpl. asimpl. 
 rewrite project_ren //=.
-have :  eguarded 0 (projectT p g) [eEVar 0 .: sigma >> (⟨g ↑ ⟩ >> projectT p)] = false. 
+have :  eguarded 0 (trans p g) [eEVar 0 .: sigma >> (⟨g ↑ ⟩ >> trans p)] = false. 
 apply/negP=>HH. move : H0.  move/negP=>H2. apply H2. 
 eapply (@eguarded_sig2 _ _ EVar)  in HH.  move : HH. asimpl. done. 
 case. simpl. done. 
@@ -358,7 +367,7 @@ Qed.
 
 (*We need guarded false implies funf = var here*)
 (*full_unf_com also*)
-Lemma proj_eq : forall p g, full_eunf (projectT p g) = full_eunf (projectT p (unf g)).  
+Lemma proj_eq : forall p g, full_eunf (trans p g) = full_eunf (trans p (unf g)).  
 Proof. 
 intros. destruct g;try done;simpl;auto. 
 case_if. simpl. rewrite full_eunf_subst.   rewrite project_subst. 
@@ -369,14 +378,14 @@ rewrite full_unf_com. rewrite H. asimpl. done.
 case.  done. simpl.  done. 
 Qed.
 
-Theorem proj_eq_full : forall p g, full_eunf (projectT p g) = full_eunf (projectT p (full_unf g)).  
+Theorem proj_eq_full : forall p g, full_eunf (trans p g) = full_eunf (trans p (full_unf g)).  
 Proof. 
 intros. 
 rewrite /full_unf. remember (mu_height g). clear Heqn. 
 elim : n g;try done. intros. rewrite iterS. rewrite -proj_eq. eauto. 
 Qed.
 
-Lemma project_project : forall p g e, Project g p e -> EQ2 e (projectT p g). 
+Lemma project_project : forall p g e, Project g p e -> EQ2 e (trans p g). 
 Proof. 
 move => p. pcofix CIH. intros. 
 apply part_of2_or_end in H0 as H0'. destruct H0'.
@@ -460,17 +469,263 @@ Qed.
 
 Lemma project_complete : forall g p e, Project g p e -> exists e', EQ2 e e' /\ project g p = Some e'.
 Proof. intros. 
-exists (projectT p g). ssa. apply project_project=>//=. 
+exists (trans p g). ssa. apply project_project=>//=. 
 rewrite /project. eapply Project_EQ2 in H.  2 : apply/project_project;eauto.  move/projectb_iff : H=>->//=. 
 Qed. 
 
 
+Lemma EQ2_EQ : forall e0 e1, EQ2 e0 e1 -> paco2 EQ_gen bot2 (etocoind e0) (etocoind e1).
+Proof. 
+pcofix CIH. intros.  punfold H0. inv H0. 
+rewrite etocoind_full_eunf. rewrite (etocoind_full_eunf e1). inv H;seq. pfold. con. 
+pfold. con. pc. eauto. 
+pfold. con. clear H1 H2.  apply/Forall_ForallC. rewrite !size_map //=. elim : es0 es1 H3 H4. case=>//=.
+move=> a l IH []//=. move => a0 l0 [] Heq. intros. inv H4. pclearbot. simpl in *. con;eauto. 
+Qed.
+
+
+
+
+Lemma CProj_Unravel : forall p g gc ec, Unravelg2 g gc ->  CProject gc p ec -> paco2 EQ_gen bot2 ec (etocoind (trans p g)). 
+Proof. 
+move => p. pcofix CIH. 
+intros. apply part_of_or_end in H1 as H1'. destruct H1'.
+move/ICpart_of_all2_iff : H=>g0.  
+have : part_of_all2 p g. apply/g0. done. 
+clear g0=>HH. 
+elim/part_of_all2_ind2 : HH gc ec H1 H0;intros. 
+- rewrite etocoind_full_eunf. rewrite proj_eq_full H0 /=.  destruct (comp_dir p a) eqn:Heqn;try done. cbn. 
+  punfold H2. inv H2. rewrite H0 in H3. inv H3. punfold H1. inv H1;try comp_disc;pc. 
+  rewrite Heqn in H9. inv H9. pfold. seq. con=>//=. eauto. 
+  have : ~ comp_dir p a by eauto. comp_disc. 
+
+- rewrite etocoind_full_eunf. rewrite proj_eq_full H2 /=.  destruct (comp_dir p a) eqn:Heqn;try done.
+  punfold H4. inv H4. rewrite H2 in H5. inv H5;pc. punfold H3. inv H3;pc;try comp_disc. 
+  rewrite -etocoind_full_eunf.   apply/H1; eauto. 
+  rewrite -etocoind_full_eunf.   apply/H1; eauto. pfold. con;eauto. 
+
+- rewrite etocoind_full_eunf. rewrite proj_eq_full H0 /=.  destruct (comp_dir p a) eqn:Heqn;try done. cbn. 
+  punfold H2. inv H2. rewrite H0 in H3. inv H3. punfold H1. inv H1;try comp_disc;pc. injt. 
+  rewrite Heqn in H7. inv H7. pfold. seq. con.  
+  rewrite -map_comp. clear H3 H2 H1  H7 H0. apply/Forall_ForallC. rewrite size_map//=. lia. 
+  move/ForallP : H11. elim : gs ecs es H6 H9 H8. case=>//=. case=>//=.
+  move => a0 l IH.   case=>//=. move => a1 l0 [] //=. move => a2 l1 [] Heq [] Heq2. intros. 
+  inv H8. inv H11. pclearbot. simpl in *. con;eauto. 
+  have : ~ comp_dir p a by eauto. comp_disc. 
+
+- rewrite etocoind_full_eunf. rewrite proj_eq_full H2 /=.  destruct (comp_dir p a) eqn:Heqn;try done.
+  punfold H4. inv H4. rewrite H2 in H5. inv H5;pc. punfold H3. inv H3;pc;try comp_disc. injt.
+  destruct gs;try done. destruct ecs;try done. simpl. 
+  rewrite -etocoind_full_eunf. destruct ecs;try done. inv H10.  pclearbot. simpl in *. 
+  apply/H1. simpl. eauto. apply/H0.  simpl. eauto. 2 : eauto. 
+  have : g2 = g2 \/ In g2 ecs. eauto. move/H13. ssa. pclearbot. done. 
+
+  destruct gs;try done. destruct ecs;try done. simpl. seq. pfold. con.
+  rewrite -etocoind_full_eunf. simpl.
+  inv H10. destruct ecs;try done. destruct H11;try done. destruct ecs;try done.  simpl in *. inv H9.  
+  simpl in *.
+  apply/H1. simpl. eauto. apply/H0.  simpl. eauto. 2 : eauto. pfold. con. 
+  move => HH. apply H6. econstructor 4.  2 : eauto. con.  done. 
+  punfold H7. inv H7. injt. inv H14. pclearbot. done.  
+
+-  subst.  apply CProject_not_part in H1. have : ECEnd = etocoind EEnd. seq. done. 
+  move=>->. apply/paco2_mon. apply/EQ2_EQ. apply/project_project. pfold. con. con.
+  rewrite -part_of2_iff. 
+  rewrite ICpart_of_iff. eauto. eauto. 
+  rewrite -Rolling_iff. 
+  apply/Unravel_Rolling.  eauto. done.
+Qed.
+
+
+
+
+Lemma inotin : forall g i sigma, (forall n, i !=  sigma n) -> i \notin endpoint_fv2 g ⟨e sigma ⟩.
+Proof.
+elim;rewrite /=;try done;intros. rewrite !inE. specialize H with n. lia.
+apply/negP. move/mapP. case. ssa. subst. rewrite mem_filter in p. ssa. 
+destruct x;try done. ssa. apply/negP. apply/H. 2 : eauto. asimpl. intros.
+destruct n. done. ssa. asimpl. move: (H0 n).  lia. 
+apply/negP. move/flattenP. case. move=> x. rewrite -map_comp. move/mapP.  case. intros. subst. 
+apply/negP. apply/H. eauto. eauto. done. 
+Qed.
+
+Lemma econtractive2_ren : forall g sigma, injective sigma -> (forall n, n <= sigma n) ->  econtractive2  g -> econtractive2 g ⟨e sigma ⟩.
+Proof.
+elim;intros;simpl;try done. 
+asimpl. split_and. have : 0 = ( 0 .: sigma >> succn) 0. done. intros. rewrite {1}x.
+apply eguarded_ren. auto. ssa. apply/H=>//=. auto. intros. destruct n. simpl. done. ssa. asimpl. move : (H1 n). lia. ssa. ssa. 
+rewrite all_map. apply/allP. intro. intros. simpl. apply H. done.  done. done.  simpl in H2. apply (allP H2). done.
+Qed.
+
+
+Lemma econtractive2_subst : forall g sigma,econtractive2 g -> (forall n, econtractive2 (sigma n)) -> econtractive2 g [e sigma].
+Proof. 
+elim;rewrite /=;intros;try done. 
+asimpl. split_and. 
+apply/eguarded_sig2.
+instantiate (1 := (EVar 0 .: EVar  >>  ⟨e ↑ ⟩)).  asimpl. done.
+case. done. simpl. intros. apply/eguarded_fv. asimpl. apply/inotin. done.
+apply H. done.  intros. destruct n.  done. simpl. asimpl.  apply/econtractive2_ren. done. done. done.
+apply H. done.  intros. done. 
+rewrite all_map. apply/allP. intro. intros. simpl. apply H. done. apply (allP H0). done. done.
+Qed.
+
+
+
+
+
+(*Lemma emu_height_subst : forall g0 sigma, (forall n, 0 < emu_height (sigma n) -> eguarded n g0) -> econtractive2 g0 -> emu_height (g0[e sigma]) = emu_height g0.
+Proof. 
+elim; try solve [by rewrite /=];intros.
+asimpl. move : (H n). destruct (emu_height (sigma n)) eqn:Heqn. done. have : 0 < n0.+1 by lia. move => + HH. move/HH=>//=. lia. 
+simpl. f_equal. asimpl. apply H. case. rewrite //=. move=> n/=. move => HH. apply/H0. move : HH. asimpl. rewrite emu_height_ren //=. ssa. 
+Qed.*)
 
 
 
 
 
 
+
+
+Lemma econtractive_unf : forall g , econtractive2 g -> econtractive2 (eunf g). 
+Proof.
+intros. rewrite /eunf. destruct g;try done. apply/econtractive2_subst. ssa. case;done. 
+Qed.
+
+Lemma econtractive_iter_unf : forall k g , econtractive2 g -> econtractive2 (iter k eunf g). 
+Proof.
+elim;try done. intros. simpl. apply/econtractive_unf. ssa. 
+Qed.
+
+Lemma econtractive_full_eunf : forall g , econtractive2 g -> econtractive2 (full_eunf g). 
+Proof. 
+intros. rewrite /full_eunf. apply/econtractive_iter_unf. done. 
+Qed.
+
+Lemma emu_height_subst_contractive : forall g0 sigma, (forall n, 0 < emu_height (sigma n) -> eguarded n g0) -> econtractive2 g0 -> emu_height (g0[e sigma]) = emu_height g0.
+Proof. 
+elim; try solve [by rewrite /=];intros.
+asimpl. move : (H n). destruct (emu_height (sigma n)) eqn:Heqn. done. have : 0 < n0.+1 by lia. move => + HH. move/HH=>//=. lia. 
+simpl. f_equal. asimpl. apply H. case. rewrite //=. move=> n/=. move => HH. apply/H0. move : HH. asimpl. rewrite emu_height_ren //=. ssa. 
+Qed.
+
+Lemma emu_height_unf_contractive : forall g , econtractive2 g -> (emu_height g).-1 = emu_height (eunf g).
+Proof.
+move => g. rewrite /=. case : g; try solve [intros;rewrite /=;done].
+intros. rewrite /=. ssa. erewrite emu_height_subst_contractive. done. eauto. case. done. done. done. 
+Qed.
+
+Lemma emu_height_iter_unf : forall k g , econtractive2 g -> (emu_height g) - k = (emu_height (iter k eunf g)). 
+Proof.
+elim;intros. rewrite /=. lia.
+rewrite /=. have : emu_height g - n.+1 = (emu_height g - n).-1 by lia. move=>->. 
+erewrite H. rewrite emu_height_unf_contractive //=.  apply/econtractive_iter_unf.  done. done. 
+Qed.
+
+Lemma iter_eunf_not_rec : forall g k, econtractive2 g -> emu_height g <= k -> forall g', iter k eunf g <> ERec g'.
+Proof.
+intros. simpl in *. apply (emu_height_iter_unf k) in H. move : H. 
+have : emu_height g - k  = 0 by lia. move=>->. intros. destruct (iter k eunf g);try done.
+Qed.
+
+Lemma full_eunf_not_rec : forall g, econtractive2 g -> forall g', full_eunf g <> ERec g'.
+Proof.
+intros. apply/iter_eunf_not_rec. done. done. 
+Qed.
+
+Lemma to_Rollinge : forall e, (forall n, n \notin endpoint_fv2 e) -> econtractive2 e -> Rollinge e. 
+Proof. 
+pcofix CIH. 
+intros. pfold. con. remember H1 as Hcont. clear HeqHcont. 
+apply econtractive_full_eunf in H1.
+have : forall n : nat_eqType, n \notin endpoint_fv2 (full_eunf e). 
+intros. rewrite -endpoint_fv2_full_eunf. done. clear H0=>H0.
+destruct (full_eunf e) eqn:Heqn. 
+move : (H0 n). ssa. lia. con. 
+con. right. apply/CIH. ssa. ssa. 
+con. 
+ssa. 
+apply/ForallP=> x xIn. right. apply/CIH.
+intros. apply/negP=> HH. apply (negP (H0 n)). apply/flattenP. exists (endpoint_fv2 x)=>//=. 
+apply/map_f. apply/inP. done. 
+apply (allP H1). apply/inP. done.
+move : (@ full_eunf_not_rec e  Hcont e0) =>Heq. 
+exfalso. apply/Heq. done. 
+Qed.
+
+(*Lemma 11 in the paper*)
+Locate Unravele.
+Print Unravele. 
+Lemma Unraveling_of_trans : forall g p, gclosed g ->  paco2 (UnfUnravele \o Unravele2_gen) bot2 (trans p g) (etocoind (trans p g)).
+Proof. 
+intros. apply/Rolling_Unravele. apply/to_Rollinge. intros. apply/fv_proj_not=>//=.
+apply/project_econtractive2.
+Qed.
+
+(*Lemma Rolling_proj : forall p g, Rolling g -> Rollinge (trans p g). 
+Proof. 
+intros. apply/to_Rollinge. intros. apply/negP. move/fv_proj=>HH. 
+move/Rolling_no_fv : H. move/(_ n). rewrite HH //=.   
+apply/project_econtractive2. 
+Qed.*)
+
+Lemma CProject_EQ : forall p g e0 e1, CProject g p e0 -> paco2 EQ_gen bot2 e0 e1 -> CProject g p e1. 
+Proof. 
+move => p. 
+pcofix CIH. intros. apply part_of_or_end in H0 as H1'.  destruct H1'. 
+elim/part_of_all_ind2 : H e0 e1 H0 H1;intros. 
+punfold H0. inv H0;try comp_disc;pc.  punfold H1. inv H1;pc.  pfold. con=>//=. eauto. 
+have : ~ comp_dir p a. eauto. comp_disc. 
+
+punfold H2. inv H2; try comp_disc;pc. pfold. con=>//=. left.  apply/H1;eauto.  
+pfold. con=>//=. comp_disc. left. apply/H1. 2 : eauto. pfold. con. eauto. eauto. 
+
+punfold H0. inv H0;try comp_disc;pc.  punfold H1. inv H1. 
+pfold. destruct (comp_dir p a) eqn:Heqn. apply coerce_forall in H9.  
+destruct H9. ssa. subst. con=>//=.  inv H4. comp_disc.  lia. 
+eauto. 
+apply/ForallP.  move/ForallP :H7. move : H6.  inv H4. 
+clear Heqn H4 H1 H0. 
+elim : gs0 es x H5 H2. case=>//=. case=>//=. 
+move => a0 l IH. case=>//=. move => a1 l0. case=>//=. 
+move => a2 l1 [] Heq [] Heq1. intros. inv H6. inv H7. pclearbot. simpl in *. 
+con;eauto. 
+done. 
+
+punfold H1. inv H1. pfold. con.  eauto. eauto. 
+punfold H2. inv H2; try comp_disc;pc.  injt. 
+pfold. econstructor. done. eauto. intros.  ssa. left. apply/H1;eauto.  
+move/H9 : H4. ssa. pclearbot. eauto. 
+punfold H3. inv H3. pfold. con. eauto. done. 
+punfold H1. subst. 
+punfold H0. inv H0;pc. pfold. con=>//=. right. eauto. 
+pfold. econstructor;eauto. ssa. move/H3 : H4. ssa. 
+move/H3 : H4. ssa. pclearbot. right. apply/CIH. eauto. pfold. done. 
+inv H1. pfold. con. done. done. 
+Qed.
+
+
+Lemma project_complete2 : forall gc p ec g, CProject gc p ec -> Unravelg2 g gc -> exists e, Unravele2 e ec  /\ project g p = Some e. 
+Proof. 
+intros. exists (trans p g). ssa. 
+apply/Unravele_iff.
+suff : exists ec', (trans p g) << Unravele_gen >> ec'. case. 
+intros. have :  paco2 EQ_gen bot2 ec (etocoind (trans p g)). apply/CProj_Unravel. eauto. done. 
+intros. apply/Unravele_iff.  apply/Unravele_eq. apply/EQ_sym. eauto.  
+apply/Rolling_Unravele. 
+apply/Rolling_proj. apply/Unravel_Rolling. eauto.
+exists (etocoind (trans p g)).
+apply/Unravele_iff. apply/Rolling_Unravele. apply/Rolling_proj. 
+apply Unravel_Rolling in H0. done. 
+rewrite /project. case_if. done. 
+exfalso. have : ~  projectb g p (trans p g) .  destruct ( projectb g p (trans p g) );try done. 
+intros. apply / x. clear H1. 
+apply/projectb_iff.
+apply/ICProject_iff. exists gc. exists (etocoind (trans p g)). ssa.
+apply/Rolling_Unravele. apply/Rolling_proj. apply/Unravel_Rolling. eauto.
+apply/CProject_EQ. eauto. apply/CProj_Unravel. eauto. done.
+Qed.
 
 
 
